cleanup types.dfy a bit

otbn_model/spec/types.dfy
@@ -17,6 +17,9 @@ const BASE_128: int := 0x1_00000000_00000000_00000000_00000000;
 const BASE_192: int := 0x1_00000000_00000000_00000000_00000000_00000000_00000000;
 const BASE_256 : int := 0x1_00000000_00000000_00000000_00000000_00000000_00000000_00000000_00000000
 
+type uint1 = i:int | 0 <= i < 2
+type uint2 = i:int | 0 <= i < 4
+
 type uint8   = i:int | 0 <= i < 0x100
 type uint16  = i:int | 0 <= i < 0x10000
 type uint32  = i:int | 0 <= i < 0x1_0000_0000
@@ -25,52 +28,27 @@ type uint128 = i:int | 0 <= i < BASE_128
 type uint256 = i:int | 0 <= i < BASE_256
 type Bignum = uint256
 
-/////////////////
-// BitsOfByte
-/////////////////
+function method {:opaque} to_uint32(b:bv32) : uint32 { b as uint32 }
+function method {:opaque} to_bv32(w:uint32) : bv32 { w as bv32 }
 
-type uint1 = i:int | 0 <= i < 2
-type uint2 = i:int | 0 <= i < 4
-datatype BitsOfByte = BitsOfByte(lo:uint2,
-                                 mid_lo:uint2,
-                                 mid_hi:uint2,
-                                 hi:uint2)
-
-function bits_to_byte(bits:BitsOfByte) : uint8
-{
-    64 * (bits.hi as uint8) + 16 * (bits.mid_hi as uint8) + 4 * (bits.mid_lo as uint8) + (bits.lo as uint8)
-}
-
-function byte_to_bits(b:uint8) : BitsOfByte
-{
-    BitsOfByte((b % 4) as uint2, ((b / 4) % 4) as uint2, ((b / 16) % 4) as uint2, ((b / 64) % 4) as uint2)
-}
-
-/////////////////
-// Bit vectors
-/////////////////
-
-function method {:opaque} BitsToWord(b:bv32) : uint32 { b as uint32 }
-function method {:opaque} WordToBits(w:uint32) : bv32 { w as bv32 }
-
-function method {:opaque} BitsToBignum(b:bv256) : uint256 { b as uint256 }
-function method {:opaque} BignumToBits(bn:uint256) : bv256 { bn as bv256 }
+function method {:opaque} to_uint256(b:bv256) : uint256 { b as uint256 }
+function method {:opaque} to_bv256(bn:uint256) : bv256 { bn as bv256 }
 
 function method {:opaque} BoolToBits(bl:bool) : bv256
 {
 	if bl then 1 as bv256 else 0 as bv256
 }
 
-lemma {:axiom} lemma_BitsToWordToBits(b:bv32)
-    ensures WordToBits(BitsToWord(b)) == b;
+lemma {:axiom} lemma_to_uint32(b:bv32)
+    ensures to_bv32(to_uint32(b)) == b;
 
-lemma {:axiom} lemma_WordToBitsToWord(w:uint32)
-    ensures BitsToWord(WordToBits(w)) == w;
+lemma {:axiom} lemma_to_bv32(w:uint32)
+    ensures to_uint32(to_bv32(w)) == w;
 
-lemma {:axiom} lemma_BitsToBignumToBits(b:bv256)
-    ensures BignumToBits(BitsToBignum(b)) == b;
+lemma {:axiom} lemma_to_uint256(b:bv256)
+    ensures to_bv256(to_uint256(b)) == b;
 
-lemma {:axiom} lemma_BignumToBitsToBignum(bn:uint256)
-    ensures BitsToBignum(BignumToBits(bn)) == bn;
-	
+lemma {:axiom} lemma_to_bv256(bn:uint256)
+    ensures to_uint256(to_bv256(bn)) == bn;
+
 } // end module types
